proof/invariants/findBlockInKS.v
@@ -42,12 +42,30 @@ Require Import Proof.Consistency Proof.DependentTypeLemmas Proof.Hoare
                Proof.Isolation Proof.StateLib Proof.WeakestPreconditions
 			   Proof.invariants.Invariants Proof.InternalLemmas.
 Require Import Compare_dec Bool List Coq.Logic.ProofIrrelevance Lia.
+Import List.ListNotations.
+
+Fixpoint isNextKernList (s: state) (kernelsList: list paddr) (baseKern: paddr) :=
+match kernelsList with
+| nil => True
+| nextKern::nextList => lookup (CPaddr (baseKern + nextoffset)) (memory s) beqAddr = Some (PADDR nextKern)
+                        /\ isNextKernList s nextList nextKern
+end.
 
 Lemma findBlockComp  (entryaddr referenceaddr : paddr) (comparator : index) (P : state -> Prop)  :
 {{fun s  =>  P s
 						/\ isBE entryaddr s}}
 Internal.findBlockComp entryaddr referenceaddr comparator
-{{fun isMatch s => P s}}.
+{{fun isMatch s => P s
+                   /\ exists blockstart,
+                        bentryStartAddr entryaddr blockstart s
+                        /\ (indexEq comparator (CIndex 0) = true ->
+                              beqAddr blockstart referenceaddr = isMatch)
+                        /\ (indexEq comparator (CIndex 0) = false ->
+                              exists bentry,
+                                lookup entryaddr (memory s) beqAddr = Some (BE bentry)
+                                /\ paddrLe blockstart referenceaddr
+                                    && paddrLe referenceaddr (endAddr (blockrange bentry)) = isMatch)
+}}.
 Proof.
 unfold Internal.findBlockComp.
 eapply bindRev.
@@ -69,13 +87,13 @@ destruct indexEq eqn:Hcomp.
 		intros.
 		{ (** ret *)
 			eapply weaken. apply ret.
-			intros. simpl. apply H0.
+			intros. simpl. destruct H0 as [H0 Hzero]. subst zero. intuition. exists blockstart. intuition. congruence.
 		}
 	+ (* case_eq beqAddr blockstart referenceaddr = false *)
 		intros.
 		{ (** ret *)
 			eapply weaken. apply ret.
-			intros. simpl. apply H0.
+			intros. simpl. destruct H0 as [H0 Hzero]. subst zero. intuition. exists blockstart. intuition. congruence.
 		}
 - (* beqIdx comparator zero = false *)
 	eapply bindRev.
@@ -101,33 +119,49 @@ destruct indexEq eqn:Hcomp.
 		intros.
 		{ (** ret *)
 			eapply weaken. apply ret.
-			intros. simpl. apply H0.
+			intros. simpl. intuition. exists blockstart. subst zero. rewrite Hcomp in *. intuition.
+      subst aboveStart. subst belowEnd. unfold bentryEndAddr in H4.
+      destruct (lookup entryaddr (memory s) beqAddr) eqn:Hlookup; try(exfalso; congruence).
+      destruct v; try(exfalso; congruence). exists b. subst blockend. intuition.
 		}
 	+ (* case_eq aboveStart && belowEnd = false *)
 		intros.
 		{ (** ret *)
 			eapply weaken. apply ret.
-			intros. simpl. apply H0.
+			intros. simpl. intuition. exists blockstart. subst zero. rewrite Hcomp in *. intuition.
+      subst aboveStart. subst belowEnd. unfold bentryEndAddr in H4.
+      destruct (lookup entryaddr (memory s) beqAddr) eqn:Hlookup; try(exfalso; congruence).
+      destruct v; try(exfalso; congruence). exists b. subst blockend. intuition.
 		}
 Qed.
 
 Lemma findBlockInKSInStructAux n (currentidx : index)
 																(currentkernelstructure referenceaddr : paddr)
 																(compoption : index) (P : state -> Prop) :
-{{  fun s : state => P s /\ consistency s
+{{  fun s : state => P s /\ consistency1 s
 										/\ isKS currentkernelstructure s
 										/\ currentidx < kernelStructureEntriesNb
 }}
 Internal.findBlockInKSInStructAux n currentidx currentkernelstructure referenceaddr compoption
-{{fun (blockaddr : paddr) (s : state) => P s /\ consistency s /\
+{{fun (blockaddr : paddr) (s : state) => P s /\ consistency1 s /\
 		(blockaddr = nullAddr
 				\/ (exists entry, lookup blockaddr s.(memory) beqAddr = Some (BE entry)
 					/\ bentryPFlag blockaddr true s
-					/\ exists finalidx, (In blockaddr (filterOptionPaddr(getKSEntriesInStructAux (maxIdx+1)
+					/\ (exists finalidx, (In blockaddr (filterOptionPaddr(getKSEntriesInStructAux (maxIdx+1)
 																								currentkernelstructure
 																								s
 																								finalidx))
-										/\ finalidx < kernelStructureEntriesNb)
+										/\ finalidx < kernelStructureEntriesNb))
+          /\ exists blockstart: paddr,
+                  bentryStartAddr blockaddr blockstart s
+                  /\ (indexEq compoption (CIndex 0) = true ->
+                        beqAddr blockstart referenceaddr = true)
+                  /\ (indexEq compoption (CIndex 0) = false ->
+                        exists bentry idx,
+                          lookup (CPaddr (currentkernelstructure + blkoffset + idx)) (memory s) beqAddr
+                            = Some (BE bentry)
+                          /\ paddrLe blockstart referenceaddr
+                              && paddrLe referenceaddr (endAddr (blockrange bentry)) = true)
 ))
 }}.
 Proof.
@@ -145,10 +179,10 @@ induction n.
 	eapply bindRev.
 	{ (** getBlockEntryAddrFromKernelStructureStart *)
 		eapply weaken. apply getBlockEntryAddrFromKernelStructureStart.
-		intros. split. apply H. unfold consistency in *. unfold consistency1 in *.
+		intros. split. apply H. unfold consistency1 in *.
 		cbn. intuition.
 	}
-	intro entryaddr.
+	intro entryaddr. simpl.
 	eapply bindRev.
 	{ (** MAL.readBlockPresentFromBlockEntryAddr *)
 		eapply weaken. apply readBlockPresentFromBlockEntryAddr.
@@ -167,6 +201,11 @@ induction n.
 		{ (** ret *)
 			eapply weaken. apply ret.
 			intros. simpl. intuition. right.
+			assert(HmatchTrue : matchcomp = true).
+			{
+				rewrite andb_true_iff in *. intuition.
+			}
+			rewrite HmatchTrue in *.
 			assert(HBEentryaddr : isBE entryaddr s)
 				by intuition.
 			apply isBELookupEq in HBEentryaddr.
@@ -177,41 +216,44 @@ induction n.
 				rewrite andb_true_iff in *. intuition.
 			}
 			rewrite HpresentTrue in *. intuition.
-			exists currentidx.
-			assert(HmaxIdx : maxIdx + 1 = S maxIdx) by (apply MaxIdxNextEq).
-			rewrite HmaxIdx. simpl.
-			unfold Paddr.addPaddrIdx.
-			simpl in *. rewrite PeanoNat.Nat.add_0_r in *.
-			unfold CPaddr in *.
-			destruct (le_dec (currentkernelstructure + currentidx) maxAddr) ; intuition.
-			-	assert(HpEq : ADT.CPaddr_obligation_1 (currentkernelstructure + currentidx) l =
-										StateLib.Paddr.addPaddrIdx_obligation_1 currentkernelstructure
-               currentidx l).
-				{ apply proof_irrelevance. }
-				rewrite HpEq in *.
-				subst entryaddr.
-				rewrite Hlookups in *.
-				destruct (beqIdx currentidx zero) eqn:beqcurrIdxZero.
-				-- simpl. left. trivial.
-				-- unfold beqIdx in beqcurrIdxZero. rewrite PeanoNat.Nat.eqb_neq in beqcurrIdxZero.
-						destruct (StateLib.Index.pred currentidx) eqn:HpredIdx ; intuition.
-						simpl. left. trivial.
-						unfold StateLib.Index.pred in *.
-						destruct (gt_dec currentidx 0) ; try(exfalso ; congruence).
-						unfold zero in *. unfold CIndex in *. destruct (le_dec 0 maxIdx) ; intuition.
-						simpl in *. lia. (* contradiction *)
-			- destruct entryaddr. simpl in *.
-				inversion H0 as [Heq]. (* {| p := p; Hp := Hp |} =
-										{| p := 0; Hp := ADT.CPaddr_obligation_2 |}*)
-				subst p.
-				assert(HnullAddrExistss : nullAddrExists s)
-						by (unfold consistency in * ; unfold consistency1 in * ; intuition).
-				unfold nullAddrExists in *. unfold isPADDR in *. unfold nullAddr in *.
-				unfold CPaddr in *. destruct (le_dec 0 maxAddr) ; intuition.
-				assert(HpEq : Hp = ADT.CPaddr_obligation_1 0 l ).
-				{ apply proof_irrelevance. }
-				rewrite <- HpEq in *.
-				rewrite Hlookups in *. congruence.
+			- exists currentidx.
+			  assert(HmaxIdx : maxIdx + 1 = S maxIdx) by (apply MaxIdxNextEq).
+			  rewrite HmaxIdx. simpl.
+			  unfold Paddr.addPaddrIdx.
+			  simpl in *. rewrite PeanoNat.Nat.add_0_r in *.
+			  unfold CPaddr in *.
+			  destruct (le_dec (currentkernelstructure + currentidx) maxAddr) ; intuition.
+			  +	assert(HpEq : ADT.CPaddr_obligation_1 (currentkernelstructure + currentidx) l =
+										  StateLib.Paddr.addPaddrIdx_obligation_1 currentkernelstructure
+                 currentidx l).
+				  { apply proof_irrelevance. }
+				  rewrite HpEq in *.
+				  subst entryaddr.
+				  rewrite Hlookups in *.
+				  destruct (beqIdx currentidx zero) eqn:beqcurrIdxZero.
+				  -- simpl. left. trivial.
+				  -- unfold beqIdx in beqcurrIdxZero. rewrite PeanoNat.Nat.eqb_neq in beqcurrIdxZero.
+						  destruct (StateLib.Index.pred currentidx) eqn:HpredIdx ; intuition.
+						  simpl. left. trivial.
+						  unfold StateLib.Index.pred in *.
+						  destruct (gt_dec currentidx 0) ; try(exfalso ; congruence).
+						  unfold zero in *. unfold CIndex in *. destruct (le_dec 0 maxIdx) ; intuition.
+						  simpl in *. lia. (* contradiction *)
+			  + destruct entryaddr. simpl in *.
+				  inversion H1 as [Heq]. (* {| p := p; Hp := Hp |} =
+										  {| p := 0; Hp := ADT.CPaddr_obligation_2 |}*)
+				  subst p.
+				  assert(HnullAddrExistss : nullAddrExists s)
+						  by (unfold consistency1 in * ; intuition).
+				  unfold nullAddrExists in *. unfold isPADDR in *. unfold nullAddr in *.
+				  unfold CPaddr in *. destruct (le_dec 0 maxAddr) ; intuition.
+				  assert(HpEq : Hp = ADT.CPaddr_obligation_1 0 l ).
+				  { apply proof_irrelevance. }
+				  rewrite <- HpEq in *.
+				  rewrite Hlookups in *. congruence.
+      - subst entryaddr. destruct H2 as [blockstart Hblockstart]. exists blockstart. intuition.
+        unfold bentryStartAddr in H1.
+        destruct H10 as [bentryBis Hbentry]. exists bentryBis. exists currentidx. intuition.
 		}
 	+ (* case_eq ispresent && matchcomp = false *)
 		intros.
@@ -227,7 +269,7 @@ induction n.
 			intros. simpl. split. apply H0. intuition.
 			apply PeanoNat.Nat.lt_le_incl.
 			rewrite KSEntriesNbLessThanMaxIdx in *.
-			apply PeanoNat.Nat.lt_add_lt_sub_l in H8.
+			apply PeanoNat.Nat.lt_add_lt_sub_l in H9.
 			rewrite PeanoNat.Nat.add_comm. assumption.
 		}
 		intro nextidx.
@@ -269,14 +311,28 @@ Qed.
 
 Lemma findBlockInKSAux n (currentkernelstructure idblock : paddr)
 																(compoption : index) (P : state -> Prop) :
-{{  fun s : state => P s /\ consistency s
+{{  fun s : state => P s /\ consistency1 s
 										/\ isKS currentkernelstructure s}}
 Internal.findBlockInKSAux n currentkernelstructure idblock compoption
-{{fun (blockaddr : paddr) (s : state) => P s /\ consistency s /\
-(blockaddr = nullAddr \/
+{{fun (blockaddr : paddr) (s : state) => P s /\ consistency1 s /\
+((blockaddr = nullAddr
+  (*/\ (exists kernList, isListOfKernelsAux kernList currentkernelstructure s
+        /\ length kernList >= n)*))
+ \/
 	(exists entry, lookup blockaddr s.(memory) beqAddr = Some (BE entry)
 		/\ bentryPFlag blockaddr true s
 		/\  (In blockaddr (filterOptionPaddr(getKSEntriesAux n currentkernelstructure s )))
+    /\ exists blockstart : paddr,
+            bentryStartAddr blockaddr blockstart s
+            /\ (indexEq compoption (CIndex 0) = true ->
+                    beqAddr blockstart idblock = true)
+            /\ (indexEq compoption (CIndex 0) = false ->
+                  exists (kernelsList firstKernList: list paddr) (lastElem: paddr) (idx: nat)
+                      (bentry: BlockEntry),
+                    isNextKernList s kernelsList currentkernelstructure
+                    /\ currentkernelstructure::kernelsList = firstKernList++[lastElem]
+                    /\ lookup (CPaddr (lastElem + blkoffset + idx)) (memory s) beqAddr = Some (BE bentry)
+                    /\ paddrLe blockstart idblock && paddrLe idblock (endAddr (blockrange bentry)) = true)
 	)
 )
 }}.
@@ -288,7 +344,8 @@ induction n.
 	intros;simpl.
 	(* MALInternal.getNullAddr *)
 	eapply weaken. unfold MALInternal.getNullAddr.
-	eapply WP.ret. intros. simpl. intuition.
+	eapply WP.ret. intros. simpl. intuition. (*left. split. reflexivity. exists []. unfold isListOfKernelsAux.
+  intuition.*)
 - (* n = S n*)
 	unfold Internal.findBlockInKSAux.
 	intros.
@@ -320,7 +377,7 @@ induction n.
 		eapply bindRev.
 		{ (** MAL.readNextFromKernelStructureStart *)
 			eapply weaken. apply readNextFromKernelStructureStart.
-			intros. simpl. split. apply H0. unfold consistency in *.
+			intros. simpl. split. apply H0. unfold consistency1 in *.
 			unfold consistency1 in *. intuition.
 		}
 		intro nextkernelstructure.
@@ -356,7 +413,7 @@ induction n.
 						destruct H4. (* exists offset : paddr, ...*)
 						intuition.
 						assert(HnextKSIsKS : NextKSIsKS s)
-							by (unfold consistency in * ; unfold consistency1 in * ; intuition).
+							by (unfold consistency1 in * ; intuition).
 						unfold NextKSIsKS in *.
 						subst x0.
 						apply HnextKSIsKS with 	(addr:=currentkernelstructure)
@@ -371,7 +428,7 @@ induction n.
 						destruct H4. (* exists offset : paddr, ...*)
 						intuition.
 						assert(HnextKSIsKS : NextKSIsKS s)
-							by (unfold consistency in * ; unfold consistency1 in * ; intuition).
+							by (unfold consistency1 in * ; intuition).
 						unfold NextKSIsKS in *.
 						subst x0.
 						apply HnextKSIsKS with 	(addr:=currentkernelstructure)
@@ -389,106 +446,121 @@ induction n.
 					destruct H11 as [aentry Ha]. (*exists entry : BlockEntry,
 												lookup a (memory s) beqAddr = Some (BE entry) ...*)
 					exists aentry. intuition.
-					subst.
-					destruct H6 as [offset Hoffset]. (*exists offset : paddr,
-														(offset = CPaddr ...*)
-					destruct Hoffset as [Hoffset HnextKSentry].
-					destruct Hoffset as [Hoffset HnextKSaddr].
-					assert(HNextKSOffsetIsPADDR : NextKSOffsetIsPADDR s)
-						by (unfold consistency in * ; unfold consistency1 in * ; intuition).
-					unfold NextKSOffsetIsPADDR in *.
-					assert(HisKScurr : isKS currentkernelstructure s) by intuition.
-					specialize (HNextKSOffsetIsPADDR currentkernelstructure
-													(CPaddr (currentkernelstructure + nextoffset))
-													HisKScurr).
-					assert(HNextKSIsKS : NextKSIsKS s)
-							by (unfold consistency in * ; unfold consistency1 in * ; intuition).
-					unfold NextKSIsKS in *.
-					specialize (HNextKSIsKS currentkernelstructure
-														(CPaddr (currentkernelstructure + nextoffset))).
-					unfold nextKSAddr in *.
-					unfold isKS in *.
-					destruct (lookup currentkernelstructure (memory s) beqAddr) eqn:Hlookupcurr ; try(exfalso ; congruence).
-					destruct v ; try(exfalso ; congruence).
-					unfold isPADDR in *.
-					intuition.
-					unfold nextKSentry in *. subst.
+          -- subst.
+					  destruct H6 as [offset Hoffset]. (*exists offset : paddr,
+														  (offset = CPaddr ...*)
+					  destruct Hoffset as [Hoffset HnextKSentry].
+					  destruct Hoffset as [Hoffset HnextKSaddr].
+					  assert(HNextKSOffsetIsPADDR : NextKSOffsetIsPADDR s)
+						  by (unfold consistency1 in * ; intuition).
+					  unfold NextKSOffsetIsPADDR in *.
+					  assert(HisKScurr : isKS currentkernelstructure s) by intuition.
+					  specialize (HNextKSOffsetIsPADDR currentkernelstructure
+													  (CPaddr (currentkernelstructure + nextoffset))
+													  HisKScurr).
+					  assert(HNextKSIsKS : NextKSIsKS s)
+							  by (unfold consistency1 in * ; intuition).
+					  unfold NextKSIsKS in *.
+					  specialize (HNextKSIsKS currentkernelstructure
+														  (CPaddr (currentkernelstructure + nextoffset))).
+					  unfold nextKSAddr in *.
+					  unfold isKS in *.
+					  destruct (lookup currentkernelstructure (memory s) beqAddr) eqn:Hlookupcurr
+                  ; try(exfalso ; congruence).
+					  destruct v ; try(exfalso ; congruence).
+					  unfold isPADDR in *.
+					  intuition.
+					  unfold nextKSentry in *. subst.
 
-					unfold Paddr.addPaddrIdx.
-					unfold CPaddr in *.
-					simpl in *.
-					destruct (le_dec (currentkernelstructure + nextoffset) maxAddr) eqn:Hnextoffset ; try lia.
-					---	(* nextaddr is well formed *)
-						assert(HpEq : ADT.CPaddr_obligation_1 (currentkernelstructure + nextoffset) l =
-												StateLib.Paddr.addPaddrIdx_obligation_1 currentkernelstructure
-									nextoffset l).
-						{ apply proof_irrelevance. }
-						rewrite HpEq in *.
+					  unfold Paddr.addPaddrIdx.
+					  unfold CPaddr in *.
+					  simpl in *.
+					  destruct (le_dec (currentkernelstructure + nextoffset) maxAddr) eqn:Hnextoffset ; try lia.
+					  ---	(* nextaddr is well formed *)
+						  assert(HpEq : ADT.CPaddr_obligation_1 (currentkernelstructure + nextoffset) l =
+												  StateLib.Paddr.addPaddrIdx_obligation_1 currentkernelstructure
+									  nextoffset l).
+						  { apply proof_irrelevance. }
+						  rewrite HpEq in *.
 
-						destruct (lookup
-										{|
-										p := currentkernelstructure + nextoffset;
-										Hp :=
-											StateLib.Paddr.addPaddrIdx_obligation_1 currentkernelstructure
-											nextoffset l
-										|} (memory s) beqAddr) eqn:Hlookupnext ; intuition.
-												destruct v ; intuition.
+						  destruct (lookup
+										  {|
+										  p := currentkernelstructure + nextoffset;
+										  Hp :=
+											  StateLib.Paddr.addPaddrIdx_obligation_1 currentkernelstructure
+											  nextoffset l
+										  |} (memory s) beqAddr) eqn:Hlookupnext ; intuition.
+												  destruct v ; intuition.
 
-						specialize (HNextKSIsKS	p HisKScurr).
-						intuition.
-						subst.
+						  specialize (HNextKSIsKS	p HisKScurr).
+						  intuition.
+						  subst.
 
-						destruct (beqAddr p nullAddr) eqn:beqpNull.
-						---- (* p = nullAddr *)
-								(* there is no following struct *)
-								rewrite <- DependentTypeLemmas.beqAddrTrue in beqpNull.
-								rewrite beqpNull in *.
+						  destruct (beqAddr p nullAddr) eqn:beqpNull.
+						  ---- (* p = nullAddr *)
+								  (* there is no following struct *)
+								  rewrite <- DependentTypeLemmas.beqAddrTrue in beqpNull.
+								  rewrite beqpNull in *.
 
-								assert(HnullAddrExists : nullAddrExists s)
-									by (unfold consistency in * ; unfold consistency1 in * ; intuition).
-								unfold nullAddrExists in *. unfold isPADDR in *.
+								  assert(HnullAddrExists : nullAddrExists s)
+									  by (unfold consistency1 in * ; intuition).
+								  unfold nullAddrExists in *. unfold isPADDR in *.
 
-								destruct (lookup nullAddr (memory s) beqAddr) eqn:Hlookupp ; intuition ; try(exfalso ; congruence).
-						---- (* p <> nullAddr *)
-								(* DUP *)
-								rewrite <- beqAddrFalse in beqpNull.
-								intuition.
+								  destruct (lookup nullAddr (memory s) beqAddr) eqn:Hlookupp ; intuition;
+                        try(exfalso ; congruence).
+						  ---- (* p <> nullAddr *)
+								  (* DUP *)
+								  rewrite <- beqAddrFalse in beqpNull.
+								  intuition.
 
-								assert(maxNbPrepare > 0)
-									by apply maxNbPrepareNotZero.
-								
-								assert(CIndex maxNbPrepare > MALInternal.zero).
-								{
-									unfold MALInternal.zero.
-									unfold CIndex.
-									destruct (le_dec 0 maxIdx) ; intuition.
-									assert(maxNbPrepare < maxIdx-1)
-										by apply maxNbPrepareNbLessThanMaxIdx.
-									destruct (le_dec maxNbPrepare maxIdx) ; intuition ; try lia.
-								}
-								unfold StateLib.Index.leb.
-								destruct (PeanoNat.Nat.leb (CIndex maxNbPrepare) MALInternal.zero) eqn:Hcong ; intuition ; try lia.
-								rewrite PeanoNat.Nat.leb_le in *. lia.
+								  assert(maxNbPrepare > 0)
+									  by apply maxNbPrepareNotZero.
+								  
+								  assert(CIndex maxNbPrepare > MALInternal.zero).
+								  {
+									  unfold MALInternal.zero.
+									  unfold CIndex.
+									  destruct (le_dec 0 maxIdx) ; intuition.
+									  assert(maxNbPrepare < maxIdx-1)
+										  by apply maxNbPrepareNbLessThanMaxIdx.
+									  destruct (le_dec maxNbPrepare maxIdx) ; intuition ; try lia.
+								  }
+								  unfold StateLib.Index.leb.
+								  destruct (PeanoNat.Nat.leb (CIndex maxNbPrepare) MALInternal.zero) eqn:Hcong ; intuition;
+                        try lia.
+								  rewrite PeanoNat.Nat.leb_le in *. lia.
 
-								destruct (lookup p (memory s) beqAddr) eqn:Hlookupp ; intuition.
-								destruct v ; intuition.
-								rewrite filterOptionPaddrSplit.
-								rewrite in_app_iff. right.
-								simpl.
-								intuition.
-								--- (* false *)
-								unfold nullAddr in *.
-								unfold CPaddr in *.
-								destruct (le_dec 0 maxAddr) ; intuition.
-								assert(HpEq : ADT.CPaddr_obligation_2 =
-										ADT.CPaddr_obligation_1 0 l)
-									by apply proof_irrelevance.
-								rewrite HpEq in *.
-								congruence.
+								  destruct (lookup p (memory s) beqAddr) eqn:Hlookupp ; intuition.
+								  destruct v ; intuition.
+								  rewrite filterOptionPaddrSplit.
+								  rewrite in_app_iff. right.
+								  simpl.
+								  intuition.
+								  --- (* false *)
+								  unfold nullAddr in *.
+								  unfold CPaddr in *.
+								  destruct (le_dec 0 maxAddr) ; intuition.
+								  assert(HpEq : ADT.CPaddr_obligation_2 =
+										  ADT.CPaddr_obligation_1 0 l)
+									  by apply proof_irrelevance.
+								  rewrite HpEq in *.
+								  congruence.
+          -- destruct H15 as [blockstart Hprops]. exists blockstart. intuition.
+             destruct H18 as [nextKernelList (firstNextKernList & (kernelStructure & (idx & (bentry &Hprops))))].
+             set(kernelsList:= nextkernelstructure::nextKernelList).
+             set(firstKernList:= currentkernelstructure::firstNextKernList).
+             exists kernelsList. exists firstKernList. exists kernelStructure. exists idx. exists bentry.
+             destruct Hprops as [HisNext (Hfirst & (HlookupKern & Hrange))]. intuition.
+             ++ subst kernelsList. simpl. destruct H6 as [offset ((Hoffset & HcurrKern) & HnextKern)].
+                subst offset. unfold nextKSentry in HnextKern.
+                destruct (lookup (CPaddr (currentkernelstructure + nextoffset)) (memory s) beqAddr)
+                      eqn:HlookupCurr; try(exfalso; congruence).
+                destruct v; try(exfalso; congruence). subst p. intuition.
+             ++ subst kernelsList. subst firstKernList. simpl. f_equal. assumption.
 				* (* impossible, foundblock is null *)
 					rewrite <- DependentTypeLemmas.beqAddrTrue in *.
 					subst.
-					unfold consistency in *. unfold consistency1 in *.
+					unfold consistency1 in *.
 					unfold nullAddrExists in *.
 					intuition. unfold isPADDR in *.
 					destruct H5 as [bentryNull (HlookupNull & _)].
@@ -503,199 +575,207 @@ induction n.
 			destruct H6 as [bentry Hbentry]. (*exists entry : BlockEntry,
 											lookup foundblock (memory s) beqAddr = ...*)
 			exists bentry. intuition.
-			destruct H9 as [finalidx HBlockInStructAux]. (*exists finalidx : index, ...*)
-			assert(HNextKSOffsetIsPADDR : NextKSOffsetIsPADDR s)
-						by (unfold consistency in * ; unfold consistency1 in * ; intuition).
-					unfold NextKSOffsetIsPADDR in *.
-					assert(HisKScurr : isKS currentkernelstructure s) by intuition.
-					specialize (HNextKSOffsetIsPADDR currentkernelstructure
-													(CPaddr (currentkernelstructure + nextoffset))
-													HisKScurr).
-					assert(HNextKSIsKS : NextKSIsKS s)
-							by (unfold consistency in * ; unfold consistency1 in * ; intuition).
-					unfold NextKSIsKS in *.
-					specialize (HNextKSIsKS currentkernelstructure
-														(CPaddr (currentkernelstructure + nextoffset))).
-					unfold nextKSAddr in *.
-					unfold isKS in *.
-					destruct (lookup currentkernelstructure (memory s) beqAddr) eqn:Hlookupcurr ; try(exfalso ; congruence).
-					destruct v ; try(exfalso ; congruence).
-					unfold isPADDR in *.
-					intuition.
-					unfold nextKSentry in *. subst.
-					unfold Paddr.addPaddrIdx.
-					unfold CPaddr in *.
-					simpl in *.
-					destruct (le_dec (currentkernelstructure + nextoffset) maxAddr) eqn:Hnextoffset ; try lia.
-					---	(* nextaddr is well formed *)
-						assert(HpEq : ADT.CPaddr_obligation_1 (currentkernelstructure + nextoffset) l =
-												StateLib.Paddr.addPaddrIdx_obligation_1 currentkernelstructure
-									nextoffset l).
-						{ apply proof_irrelevance. }
-						rewrite HpEq in *.
+      *	destruct H6 as [finalidx HBlockInStructAux]. (*exists finalidx : index, ...*)
+			  assert(HNextKSOffsetIsPADDR : NextKSOffsetIsPADDR s)
+						  by (unfold consistency1 in * ; intuition).
+					  unfold NextKSOffsetIsPADDR in *.
+					  assert(HisKScurr : isKS currentkernelstructure s) by intuition.
+					  specialize (HNextKSOffsetIsPADDR currentkernelstructure
+													  (CPaddr (currentkernelstructure + nextoffset))
+													  HisKScurr).
+					  assert(HNextKSIsKS : NextKSIsKS s)
+							  by (unfold consistency1 in * ; intuition).
+					  unfold NextKSIsKS in *.
+					  specialize (HNextKSIsKS currentkernelstructure
+														  (CPaddr (currentkernelstructure + nextoffset))).
+					  unfold nextKSAddr in *.
+					  unfold isKS in *.
+					  destruct (lookup currentkernelstructure (memory s) beqAddr) eqn:Hlookupcurr;
+                  try(exfalso; congruence).
+					  destruct v ; try(exfalso ; congruence).
+					  unfold isPADDR in *.
+					  intuition.
+					  unfold nextKSentry in *. subst.
+					  unfold Paddr.addPaddrIdx.
+					  unfold CPaddr in *.
+					  simpl in *.
+					  destruct (le_dec (currentkernelstructure + nextoffset) maxAddr) eqn:Hnextoffset ; try lia.
+					  ---	(* nextaddr is well formed *)
+						  assert(HpEq : ADT.CPaddr_obligation_1 (currentkernelstructure + nextoffset) l =
+												  StateLib.Paddr.addPaddrIdx_obligation_1 currentkernelstructure
+									  nextoffset l).
+						  { apply proof_irrelevance. }
+						  rewrite HpEq in *.
 
-						destruct (lookup
-										{|
-										p := currentkernelstructure + nextoffset;
-										Hp :=
-											StateLib.Paddr.addPaddrIdx_obligation_1 currentkernelstructure
-											nextoffset l
-										|} (memory s) beqAddr) eqn:Hlookupnext ; intuition.
-												destruct v ; intuition.
+						  destruct (lookup
+										  {|
+										  p := currentkernelstructure + nextoffset;
+										  Hp :=
+											  StateLib.Paddr.addPaddrIdx_obligation_1 currentkernelstructure
+											  nextoffset l
+										  |} (memory s) beqAddr) eqn:Hlookupnext ; intuition.
+												  destruct v ; intuition.
 
-						specialize (HNextKSIsKS	p HisKScurr).
-						intuition.
-						subst.
+						  specialize (HNextKSIsKS	p HisKScurr).
+						  intuition.
+						  subst.
 
-						destruct (beqAddr p nullAddr) eqn:beqpNull.
-						---- (* p = nullAddr *)
-								(* there is no following struct *)
-								rewrite <- DependentTypeLemmas.beqAddrTrue in beqpNull.
-								rewrite beqpNull in *.
+						  destruct (beqAddr p nullAddr) eqn:beqpNull.
+						  ---- (* p = nullAddr *)
+								  (* there is no following struct *)
+								  rewrite <- DependentTypeLemmas.beqAddrTrue in beqpNull.
+								  rewrite beqpNull in *.
 
-								assert(HnullAddrExists : nullAddrExists s)
-									by (unfold consistency in * ; unfold consistency1 in * ; intuition).
-								unfold nullAddrExists in *. unfold isPADDR in *.
+								  assert(HnullAddrExists : nullAddrExists s)
+									  by (unfold consistency1 in * ; intuition).
+								  unfold nullAddrExists in *. unfold isPADDR in *.
 
-								destruct (lookup nullAddr (memory s) beqAddr) eqn:Hlookupp ; intuition ; try(exfalso ; congruence).
-								destruct v ; intuition.
-								subst p.
-								(* DUP *)
-								eapply getKSEntriesInStructAuxInside with (idx := finalidx)(n:=(maxIdx + 1))(m:= (maxIdx+1))  ; intuition ; try lia.
-								+++ unfold isKS. rewrite Hlookupcurr. assumption.
-								+++ destruct finalidx.
-									assert(HidxEq : CIndex 7 = CIndex (kernelStructureEntriesNb-1)).
-									{
-										unfold CIndex. simpl in *.
-										destruct (le_dec 7 maxIdx) ; trivial.
-									}
-									rewrite HidxEq.
-									unfold CIndex.
-									assert(kernelStructureEntriesNb < maxIdx-1)
-										by (apply KSEntriesNbLessThanMaxIdx).
-									destruct (le_dec (kernelStructureEntriesNb - 1) maxIdx) ; intuition ; try lia.
-								+++ assert(HidxEq : CIndex 7 = CIndex (kernelStructureEntriesNb-1)).
-									{
-										unfold CIndex. simpl in *.
-										destruct (le_dec 7 maxIdx) ; trivial.
-									}
-									rewrite HidxEq.
-									unfold CIndex.
-									assert(kernelStructureEntriesNb < maxIdx-1)
-										by (apply KSEntriesNbLessThanMaxIdx).
-									destruct (le_dec (kernelStructureEntriesNb-1) maxIdx) ; intuition ; simpl ; try lia.
-									simpl in *. lia.
-								+++ assert(HidxEq : CIndex 7 = CIndex (kernelStructureEntriesNb-1)).
-									{
-										unfold CIndex. simpl in *.
-										destruct (le_dec 7 maxIdx) ; trivial.
-									}
-									rewrite HidxEq.
-									unfold CIndex.
-									assert(kernelStructureEntriesNb < maxIdx-1)
-										by (apply KSEntriesNbLessThanMaxIdx).
-									destruct (le_dec (kernelStructureEntriesNb-1) maxIdx) ; intuition ; simpl ; try lia.
-									simpl in *. lia.
-								+++ assert(HidxEq : CIndex 7 = CIndex (kernelStructureEntriesNb-1)).
-									{
-										unfold CIndex. simpl in *.
-										destruct (le_dec 7 maxIdx) ; trivial.
-									}
-									rewrite HidxEq.
-									unfold CIndex.
-									assert(kernelStructureEntriesNb < maxIdx-1)
-										by (apply KSEntriesNbLessThanMaxIdx).
-									destruct (le_dec (kernelStructureEntriesNb-1) maxIdx) ; intuition ; simpl ; try lia.
-						---- (* p <> nullAddr *)
-								(* DUP *)
-								rewrite <- beqAddrFalse in beqpNull.
-								intuition.
+								  destruct (lookup nullAddr (memory s) beqAddr) eqn:Hlookupp ; intuition;
+                        try(exfalso; congruence).
+								  destruct v ; intuition.
+								  subst p.
+								  (* DUP *)
+								  eapply getKSEntriesInStructAuxInside with (idx := finalidx)(n:=(maxIdx + 1))(m:= (maxIdx+1));
+                        intuition ; try lia.
+								  +++ unfold isKS. rewrite Hlookupcurr. assumption.
+								  +++ destruct finalidx.
+									  assert(HidxEq : CIndex 7 = CIndex (kernelStructureEntriesNb-1)).
+									  {
+										  unfold CIndex. simpl in *.
+										  destruct (le_dec 7 maxIdx) ; trivial.
+									  }
+									  rewrite HidxEq.
+									  unfold CIndex.
+									  assert(kernelStructureEntriesNb < maxIdx-1)
+										  by (apply KSEntriesNbLessThanMaxIdx).
+									  destruct (le_dec (kernelStructureEntriesNb - 1) maxIdx) ; intuition ; try lia.
+								  +++ assert(HidxEq : CIndex 7 = CIndex (kernelStructureEntriesNb-1)).
+									  {
+										  unfold CIndex. simpl in *.
+										  destruct (le_dec 7 maxIdx) ; trivial.
+									  }
+									  rewrite HidxEq.
+									  unfold CIndex.
+									  assert(kernelStructureEntriesNb < maxIdx-1)
+										  by (apply KSEntriesNbLessThanMaxIdx).
+									  destruct (le_dec (kernelStructureEntriesNb-1) maxIdx) ; intuition ; simpl ; try lia.
+									  simpl in *. lia.
+								  +++ assert(HidxEq : CIndex 7 = CIndex (kernelStructureEntriesNb-1)).
+									  {
+										  unfold CIndex. simpl in *.
+										  destruct (le_dec 7 maxIdx) ; trivial.
+									  }
+									  rewrite HidxEq.
+									  unfold CIndex.
+									  assert(kernelStructureEntriesNb < maxIdx-1)
+										  by (apply KSEntriesNbLessThanMaxIdx).
+									  destruct (le_dec (kernelStructureEntriesNb-1) maxIdx) ; intuition ; simpl ; try lia.
+									  simpl in *. lia.
+								  +++ assert(HidxEq : CIndex 7 = CIndex (kernelStructureEntriesNb-1)).
+									  {
+										  unfold CIndex. simpl in *.
+										  destruct (le_dec 7 maxIdx) ; trivial.
+									  }
+									  rewrite HidxEq.
+									  unfold CIndex.
+									  assert(kernelStructureEntriesNb < maxIdx-1)
+										  by (apply KSEntriesNbLessThanMaxIdx).
+									  destruct (le_dec (kernelStructureEntriesNb-1) maxIdx) ; intuition ; simpl ; try lia.
+						  ---- (* p <> nullAddr *)
+								  (* DUP *)
+								  rewrite <- beqAddrFalse in beqpNull.
+								  intuition.
 
-								assert(maxNbPrepare > 0)
-									by apply maxNbPrepareNotZero.
-								
-								assert(CIndex maxNbPrepare > MALInternal.zero).
-								{
-									unfold MALInternal.zero.
-									unfold CIndex.
-									destruct (le_dec 0 maxIdx) ; intuition.
-									assert(maxNbPrepare < maxIdx-1)
-										by apply maxNbPrepareNbLessThanMaxIdx.
-									destruct (le_dec maxNbPrepare maxIdx) ; intuition ; try lia.
-								}
-								unfold StateLib.Index.leb.
-								destruct (PeanoNat.Nat.leb (CIndex maxNbPrepare) MALInternal.zero) eqn:Hcong ; intuition ; try lia.
-								rewrite PeanoNat.Nat.leb_le in *. lia.
+								  assert(maxNbPrepare > 0)
+									  by apply maxNbPrepareNotZero.
+								  
+								  assert(CIndex maxNbPrepare > MALInternal.zero).
+								  {
+									  unfold MALInternal.zero.
+									  unfold CIndex.
+									  destruct (le_dec 0 maxIdx) ; intuition.
+									  assert(maxNbPrepare < maxIdx-1)
+										  by apply maxNbPrepareNbLessThanMaxIdx.
+									  destruct (le_dec maxNbPrepare maxIdx) ; intuition ; try lia.
+								  }
+								  unfold StateLib.Index.leb.
+								  destruct (PeanoNat.Nat.leb (CIndex maxNbPrepare) MALInternal.zero) eqn:Hcong; intuition;
+                      try lia.
+								  rewrite PeanoNat.Nat.leb_le in *. lia.
 
-								destruct (lookup p (memory s) beqAddr) eqn:Hlookupp ; intuition.
-								destruct v ; intuition.
-								rewrite filterOptionPaddrSplit.
-								rewrite in_app_iff. left.
+								  destruct (lookup p (memory s) beqAddr) eqn:Hlookupp ; intuition.
+								  destruct v ; intuition.
+								  rewrite filterOptionPaddrSplit.
+								  rewrite in_app_iff. left.
 
-								(* DUP *)
-								eapply getKSEntriesInStructAuxInside with (idx := finalidx)(n:=(maxIdx + 1))(m:= (maxIdx+1))  ; intuition ; try lia.
-								+++ unfold isKS. rewrite Hlookupcurr. assumption.
-								+++ destruct finalidx.
-									assert(HidxEq : CIndex 7 = CIndex (kernelStructureEntriesNb-1)).
-									{
-										unfold CIndex. simpl in *.
-										destruct (le_dec 7 maxIdx) ; trivial.
-									}
-									rewrite HidxEq.
-									unfold CIndex.
-									assert(kernelStructureEntriesNb < maxIdx-1)
-										by (apply KSEntriesNbLessThanMaxIdx).
-									destruct (le_dec (kernelStructureEntriesNb - 1) maxIdx) ; intuition ; try lia.
-								+++ assert(HidxEq : CIndex 7 = CIndex (kernelStructureEntriesNb-1)).
-									{
-										unfold CIndex. simpl in *.
-										destruct (le_dec 7 maxIdx) ; trivial.
-									}
-									rewrite HidxEq.
-									unfold CIndex.
-									assert(kernelStructureEntriesNb < maxIdx-1)
-										by (apply KSEntriesNbLessThanMaxIdx).
-									destruct (le_dec (kernelStructureEntriesNb-1) maxIdx) ; intuition ; simpl ; try lia.
-									simpl in *. lia.
-								+++ assert(HidxEq : CIndex 7 = CIndex (kernelStructureEntriesNb-1)).
-									{
-										unfold CIndex. simpl in *.
-										destruct (le_dec 7 maxIdx) ; trivial.
-									}
-									rewrite HidxEq.
-									unfold CIndex.
-									assert(kernelStructureEntriesNb < maxIdx-1)
-										by (apply KSEntriesNbLessThanMaxIdx).
-									destruct (le_dec (kernelStructureEntriesNb-1) maxIdx) ; intuition ; simpl ; try lia.
-									simpl in *. lia.
-								+++ assert(HidxEq : CIndex 7 = CIndex (kernelStructureEntriesNb-1)).
-									{
-										unfold CIndex. simpl in *.
-										destruct (le_dec 7 maxIdx) ; trivial.
-									}
-									rewrite HidxEq.
-									unfold CIndex.
-									assert(kernelStructureEntriesNb < maxIdx-1)
-										by (apply KSEntriesNbLessThanMaxIdx).
-									destruct (le_dec (kernelStructureEntriesNb-1) maxIdx) ; intuition ; simpl ; try lia.
+								  (* DUP *)
+								  eapply getKSEntriesInStructAuxInside with (idx := finalidx)(n:=(maxIdx + 1))(m:= (maxIdx+1));
+                        intuition ; try lia.
+								  +++ unfold isKS. rewrite Hlookupcurr. assumption.
+								  +++ destruct finalidx.
+									  assert(HidxEq : CIndex 7 = CIndex (kernelStructureEntriesNb-1)).
+									  {
+										  unfold CIndex. simpl in *.
+										  destruct (le_dec 7 maxIdx) ; trivial.
+									  }
+									  rewrite HidxEq.
+									  unfold CIndex.
+									  assert(kernelStructureEntriesNb < maxIdx-1)
+										  by (apply KSEntriesNbLessThanMaxIdx).
+									  destruct (le_dec (kernelStructureEntriesNb - 1) maxIdx) ; intuition ; try lia.
+								  +++ assert(HidxEq : CIndex 7 = CIndex (kernelStructureEntriesNb-1)).
+									  {
+										  unfold CIndex. simpl in *.
+										  destruct (le_dec 7 maxIdx) ; trivial.
+									  }
+									  rewrite HidxEq.
+									  unfold CIndex.
+									  assert(kernelStructureEntriesNb < maxIdx-1)
+										  by (apply KSEntriesNbLessThanMaxIdx).
+									  destruct (le_dec (kernelStructureEntriesNb-1) maxIdx) ; intuition ; simpl ; try lia.
+									  simpl in *. lia.
+								  +++ assert(HidxEq : CIndex 7 = CIndex (kernelStructureEntriesNb-1)).
+									  {
+										  unfold CIndex. simpl in *.
+										  destruct (le_dec 7 maxIdx) ; trivial.
+									  }
+									  rewrite HidxEq.
+									  unfold CIndex.
+									  assert(kernelStructureEntriesNb < maxIdx-1)
+										  by (apply KSEntriesNbLessThanMaxIdx).
+									  destruct (le_dec (kernelStructureEntriesNb-1) maxIdx) ; intuition ; simpl ; try lia.
+									  simpl in *. lia.
+								  +++ assert(HidxEq : CIndex 7 = CIndex (kernelStructureEntriesNb-1)).
+									  {
+										  unfold CIndex. simpl in *.
+										  destruct (le_dec 7 maxIdx) ; trivial.
+									  }
+									  rewrite HidxEq.
+									  unfold CIndex.
+									  assert(kernelStructureEntriesNb < maxIdx-1)
+										  by (apply KSEntriesNbLessThanMaxIdx).
+									  destruct (le_dec (kernelStructureEntriesNb-1) maxIdx) ; intuition ; simpl ; try lia.
 
-					--- (* false, null is not null -> contradiction  *)
-						unfold nullAddr in *.
-						unfold CPaddr in *.
-						destruct (le_dec 0 maxAddr) ; intuition.
-						assert(HpEq : ADT.CPaddr_obligation_2 =
-								ADT.CPaddr_obligation_1 0 l)
-							by apply proof_irrelevance.
-						rewrite HpEq in *.
-						congruence.
+					  --- (* false, null is not null -> contradiction  *)
+						  unfold nullAddr in *.
+						  unfold CPaddr in *.
+						  destruct (le_dec 0 maxAddr) ; intuition.
+						  assert(HpEq : ADT.CPaddr_obligation_2 =
+								  ADT.CPaddr_obligation_1 0 l)
+							  by apply proof_irrelevance.
+						  rewrite HpEq in *.
+						  congruence.
+      * destruct H10 as [blockstart Hprops]. exists blockstart. intuition. exists []. exists [].
+        exists currentkernelstructure. destruct H13 as [bentryBis (idx & Hprops)]. exists idx. exists bentryBis.
+        unfold isNextKernList. intuition.
 	}
 Qed.
 
 
 Lemma findBelongingBlock (idPD referenceaddr: paddr) (P : state -> Prop) :
-{{ fun s => P s /\ consistency s /\ isPDT idPD s}}
+{{ fun s => P s /\ consistency1 s /\ isPDT idPD s}}
 Internal.findBelongingBlock idPD referenceaddr
-{{fun (blockaddr : paddr) (s : state) => P s /\ consistency s /\
+{{fun (blockaddr : paddr) (s : state) => P s /\ consistency1 s /\
 			(blockaddr = nullAddr
 					\/ (exists entry, lookup blockaddr s.(memory) beqAddr = Some (BE entry)
 						/\ bentryPFlag blockaddr true s))
@@ -744,8 +824,7 @@ case_eq kernelstructureisnull.
 		intros. simpl. intuition.
 		eapply H. apply H.
 		intuition.
-		right. intuition.
-		destruct H1 as [bentry (Hbentry & (HbentryPFlag & Hleft))]. (*exists entry : BlockEntry, ...*)
+		right. destruct H1 as [bentry (Hbentry & (HbentryPFlag & Hleft))]. (*exists entry : BlockEntry, ...*)
 		exists bentry. intuition.
 		intros. simpl. intuition.
 		rewrite <- beqAddrFalse in *. intuition.
@@ -754,7 +833,7 @@ case_eq kernelstructureisnull.
 		apply isPDTLookupEq in HPDT. destruct HPDT as [pdentry Hlookuppd].
 
 		assert(HStructurePointerIsKS : StructurePointerIsKS s)
-			by (unfold consistency in * ; unfold consistency1 in * ; intuition).
+			by (unfold consistency1 in * ; intuition).
 		unfold StructurePointerIsKS in *.
 		specialize (HStructurePointerIsKS idPD pdentry Hlookuppd).
 		unfold pdentryStructurePointer in *.
@@ -763,13 +842,16 @@ case_eq kernelstructureisnull.
 Qed.
 
 Lemma findBlockInKS (idPD blockEntryAddr: paddr) (P : state -> Prop) :
-{{ fun s => P s /\ consistency s /\ isPDT idPD s}}
+{{ fun s => P s /\ consistency1 s /\ isPDT idPD s}}
 Internal.findBlockInKS idPD blockEntryAddr
-{{fun (blockaddr : paddr) (s : state) => P s /\ consistency s /\
+{{fun (blockaddr : paddr) (s : state) => P s /\ consistency1 s /\
 			(blockaddr = nullAddr
 			\/ (exists entry, lookup blockaddr s.(memory) beqAddr = Some (BE entry)
-						/\ bentryPFlag blockaddr true s
-						/\ In blockaddr (getMappedBlocks idPD s) ) )
+					/\ bentryPFlag blockaddr true s
+					/\ In blockaddr (getMappedBlocks idPD s)
+          /\ exists blockstart : paddr,
+                bentryStartAddr blockaddr blockstart s
+                /\ beqAddr blockstart blockEntryAddr = true))
 }}.
 Proof.
 unfold Internal.findBlockInKS.
@@ -811,7 +893,7 @@ case_eq kernelstructureisnull.
 		apply isPDTLookupEq in HPDT. destruct HPDT as [pdentry Hlookuppd].
 
 		assert(HStructurePointerIsKS : StructurePointerIsKS s)
-			by (unfold consistency in * ; unfold consistency1 in * ; intuition).
+			by (unfold consistency1 in * ; intuition).
 		unfold StructurePointerIsKS in *.
 		specialize (HStructurePointerIsKS idPD pdentry Hlookuppd).
 		unfold pdentryStructurePointer in *.
@@ -825,28 +907,30 @@ case_eq kernelstructureisnull.
 		right.
 		destruct H6 as [bentry (Hbentry & (HbentryPFlag & Hksentries))]. (*exists entry : BlockEntry, ...*)
 		exists bentry. intuition.
-		unfold getMappedBlocks.
-		unfold getKSEntries.
-		assert(HPDT : isPDT idPD s) by assumption.
-		apply isPDTLookupEq in HPDT. destruct HPDT as [idpdentry Hlookupidpd].
-		unfold pdentryStructurePointer in *.
-		unfold isPDT in *.
-		rewrite Hlookupidpd in *.
-		subst.
-		destruct (beqAddr (structure idpdentry) nullAddr) eqn:HksNull ; trivial.
-		- 	(* (structure idpdentry) = nullAddr *)
-			(* contradiction
-				-> nulladdr cannot have a valid nextoffset *)
-			rewrite <- DependentTypeLemmas.beqAddrTrue in HksNull.
-			rewrite HksNull in *.
-			exfalso ; congruence.
-		-	(* (structure idpdentry) <> nullAddr *)
-			induction ((filterOptionPaddr (getKSEntriesAux maxNbPrepare (structure idpdentry) s))) ; simpl in * ; intuition.
-			subst.
-			unfold bentryPFlag in *. rewrite Hbentry in *.
-			destruct (present bentry) ; simpl ; try lia ; intuition.
-			destruct (lookup a0 (memory s) beqAddr) ; intuition.
-			destruct v;  intuition.
-			destruct (present b) ; intuition.
+	  - unfold getMappedBlocks.
+	    unfold getKSEntries.
+	    assert(HPDT : isPDT idPD s) by assumption.
+	    apply isPDTLookupEq in HPDT. destruct HPDT as [idpdentry Hlookupidpd].
+	    unfold pdentryStructurePointer in *.
+	    unfold isPDT in *.
+	    rewrite Hlookupidpd in *.
+	    subst.
+	    destruct (beqAddr (structure idpdentry) nullAddr) eqn:HksNull ; trivial.
+	    + 	(* (structure idpdentry) = nullAddr *)
+		    (* contradiction
+			    -> nulladdr cannot have a valid nextoffset *)
+		    rewrite <- DependentTypeLemmas.beqAddrTrue in HksNull.
+		    rewrite HksNull in *.
+		    exfalso ; congruence.
+	    +	(* (structure idpdentry) <> nullAddr *)
+		    induction ((filterOptionPaddr (getKSEntriesAux maxNbPrepare (structure idpdentry) s))) ; simpl in *;
+                intuition.
+		    subst.
+		    unfold bentryPFlag in *. rewrite Hbentry in *.
+		    destruct (present bentry) ; simpl ; try lia ; intuition.
+		    destruct (lookup a0 (memory s) beqAddr) ; intuition.
+		    destruct v;  intuition.
+		    destruct (present b) ; intuition.
+    - destruct H6 as [blockstart Hprops]. exists blockstart. subst zero. intuition.
 	}
 Qed.
